Exam Practice/Reverse.dfy
@@ -1,0 +1,19 @@
+method Reverse(arr: array<int>)
+requires arr != null
+modifies arr
+ensures forall i :: 0 <= i < arr.Length/2 ==> arr[i] == old(arr[arr.Length - 1 - i])
+ensures forall i :: 0 <= i < arr.Length/2 ==> arr[arr.Length - 1 - i] == old(arr[i])
+{
+    var count := 0;
+    while count < arr.Length / 2
+    invariant 0 <= count <= arr.Length / 2
+    invariant multiset(arr[..]) == multiset(old(arr[..]))
+    invariant forall i :: count <= i <= arr.Length - 1 - count ==> arr[i] == old(arr[i])
+    invariant forall i :: 0 <= i < count ==> arr[i] == old(arr[arr.Length - 1 - i])
+    invariant forall i :: 0 <= i < count ==> arr[arr.Length - 1 - i] == old(arr[i])
+    {
+        arr[count], arr[arr.Length - 1 - count] := arr[arr.Length - 1 - count], arr[count];
+        count := count + 1;
+    }
+}
+
